execution/tests/FA2Tests/FA2Gens.v
@@ -138,6 +138,7 @@ Definition gSingleTransfer (lc : LocalChain)
             to_ := to;
             transfer_token_id := tokenid;
             amount := amount;
+            sender_callback_addr := zero_address;
           |})
     )
   | None => returnGen None
